Xv6/SpecMain.lean
@@ -292,7 +292,7 @@ def wp_main_boot_body [IcacheG GF] [LogG GF] [FsBlocksG GF] [IregG GF] [FsTopG G
     [Fscfg] [Icfg] (X : CurCtx)
     (Γ : SchedNames) [ClaimIs (hlc := hlc) GF Γ]
     (γ0 γ1 : UartNames) (γc γl0 γl1 : GName) (γd : DiskNames) (γdl γt : GName)
-    (pd pav pu : BitVec 64) [EnvIs (hlc := hlc) GF Γ γ0 γ1 γc γl0 γl1 γd γdl γt pd pav pu]
+    (pd pav pu : BitVec 64) [EnvIs (hlc := hlc) GF Γ γ0 γ1 γc γl0 γl1 γd γdl γt]
     (cpu : CPU) (k : KCtx) (cn : ConsNames) (l0 l1 : List (BitVec 8)) (c0 : VirtioCfg)
     (dk : Nat → BitVec 8) (sb : FsSb) (nib : Nat) (cov : ExtTreeSet Nat compare) (ndisk : Nat)
     (S : FsStateRec) (Pb : Nat → List (BitVec 8))
@@ -362,7 +362,7 @@ structure MAIN : Prop where
     [Fscfg] [Icfg] (X : CurCtx)
     (Γ : SchedNames) [ClaimIs (hlc := hlc) GF Γ]
     (γ0 γ1 : UartNames) (γc γl0 γl1 : GName) (γd : DiskNames) (γdl γt : GName)
-    (pd pav pu : BitVec 64) [EnvIs (hlc := hlc) GF Γ γ0 γ1 γc γl0 γl1 γd γdl γt pd pav pu]
+    (pd pav pu : BitVec 64) [EnvIs (hlc := hlc) GF Γ γ0 γ1 γc γl0 γl1 γd γdl γt]
     (cpu : CPU) (k : KCtx) (cn : ConsNames) (l0 l1 : List (BitVec 8)) (c0 : VirtioCfg)
     (dk : Nat → BitVec 8) (sb : FsSb) (nib : Nat) (cov : ExtTreeSet Nat compare) (ndisk : Nat)
     (S : FsStateRec) (Pb : Nat → List (BitVec 8))
